\documentclass[12pt, a4paper]{article}
\setlength{\parindent}{0pt}
\usepackage{amsmath}
\usepackage{amsthm}
\usepackage{amssymb}
\usepackage[a4paper, portrait, margin=1in]{geometry}

% i like the black square better.
\renewcommand{\qedsymbol}{$\blacksquare$}
%\renewcommand{\implies}{\Rightarrow}

\newcommand{\N}{\mathbb{N}}
\newcommand{\R}{\mathbb{R}}
\newcommand{\ddx}{\frac{d}{dx}}
\newcommand{\st}{\text{ s.t. }}
\newcommand{\fn}[3]{#1 \colon #2 \to #3}

\newtheorem{theorem}{Theorem}

% let's begin
\begin{document}

\textbf{(Q3)}

\textit{(a)} Since $(f^{-1})'(f(x)) = \displaystyle{\frac{1}{f'(x)}}$,
$(f^{-1})'(4) = \displaystyle\frac{1}{f'(-1)} = 2$.

\textit{(b)} $f(0) = 1 \implies f^{-1}(1) = 0$, and $f'(0) = -1.$ Thus,
the tangent of $f$ at 0 is $-x$. Since the tangent of $f^{-1}$ is given 
by a reflection across the line $x = y$, the tangent of $f^{-1}$ at 1
is also $-x$.

\textit{(c)} $f(1) = 2 \implies f^{-1}(2) = 1$. Since $f'(1) = 0$,
the tangent line at $f^{-1}(2)$ will be vertical, and thus the derivative
will be undefined and thus not differentiable.

\end{document}