\documentclass[12pt, a4paper]{article}
\setlength{\parindent}{0pt}
\usepackage[a4paper, portrait, margin=1in]{geometry}

\usepackage{preamble}

\begin{document}

\textbf{(Q2)}

\textit{(a)}

\begin{align*}
    \int \frac{t^4 + 2t + 1}{\sqrt[3]{t}} dt & =
    \int (t^4 + 2t + 1)t^{-\frac{1}{3}} dt\\ & =
    \int t^{\frac{11}{3}} dt + 2\int t^{\frac{2}{3}} dt
    + \int t^{\frac{1}{3}} dt \\ & =
    \frac{3}{14}t^{\frac{14}{3}} + \frac{6}{5}t^{\frac{5}{3}}
    + \frac{3}{2}t^{\frac{2}{3}}
\end{align*}

\textit{(b)}

\begin{align*}
    \int (x + 1)x^{135} dx & = \int x^{136} dx + \int x^{135} dx\\
    & = \frac{1}{137}x^{137} + \frac{1}{136}x^{136}
\end{align*}

\textit{(c)} Let $u = 2 \pi x$ Then $du = 2 \pi dx$. Then we have

\[
    \int_0^1 \sin(u) du = \int_{0}^{2 \pi} \sin(2 \pi x)
    \frac{1}{2\pi} dx = \frac{-\cos(2 \pi x)}{2 \pi}
    \big\vert_0^{2 \pi} = 0
\]

\textit{(d)}

\[
    \int_{-1}^{1} (e^t + t^3) dt = (e^t + \frac{1}{4}t^4)\big\vert^1_{-1}
    = e - \frac{1}{e}
\]
\end{document}