\documentclass[12pt, a4paper]{article}
\setlength{\parindent}{0pt}
\usepackage{amsmath}
\usepackage{amsthm}
\usepackage{amssymb}
\usepackage[a4paper, portrait, margin=1in]{geometry}

\renewcommand{\qedsymbol}{$\blacksquare$}
\renewcommand{\epsilon}{\varepsilon}

\newcommand{\R}{\mathbb{R}}
\newcommand{\Z}{\mathbb{Z}}
\newcommand{\displim}[1]{\displaystyle{\lim_{#1}\:}}
\newcommand{\zerolim}{\displim{x \to 0}}
\newcommand{\st}{\text{ s.t. }}

\newtheorem{theorem}{Theorem}

% let's begin
\begin{document}
\textbf{(Q6)}

First, we manipulate the polynomial into something that is easier to work with.

Multiplying the polynomial by its conjugate:

\begin{align*}
    \sqrt{x^6 - x^3} + x^3 & =
    \frac{\sqrt{x^6 - x^3} + x^3}{1} \cdot
    \frac{\sqrt{x^6 - x^3} - x^3}{\sqrt{x^6 - x^3} - x^3}\\
    & = \frac{x^6 - x^3 - x^6}{\sqrt{x^6 - x^3} - x^3}\\
    & = \frac{- x^3}{\sqrt{x^6}\sqrt{1 - \frac{1}{x^3}} - x^3}
\end{align*}

Since we are considering limits at negative infinity,
\[
    \sqrt{x^6} = \left|x^3\right| = -x^3 \text{ for $x < 0$}
\]

It follows that:

\begin{align*}
    \frac{- x^3}{-x^3\sqrt{1 - \frac{1}{x^3}} - x^3} & =
    \frac{1}{\sqrt{1 - \frac{1}{x^3}} + 1}
\end{align*}

From which we can calculate the limit.

Since $\displim{x \to -\infty} \frac{1}{x^k} = 0$ for $k > 0$,
\[
    \displim{x \to -\infty} \sqrt{1 - 0} = \sqrt{\displim{x \to -\infty} 1} = 1
\]

From which it follows:

\begin{align*}
    \displim{x \to -\infty} \frac{1}{\sqrt{1 - \frac{1}{x^3}} + 1} & =
    \displim{x \to -\infty} \frac{1}{\sqrt{1 - 0} + 1}\\
    & = \displim{x \to -\infty} \frac{1}{1 + 1}\\
    & = \frac{1}{2}
\end{align*}

\end{document}