\documentclass[12pt, a4paper]{article}
\setlength{\parindent}{0pt}
\usepackage{amsmath}
\usepackage{amsthm}
\usepackage{amssymb}
\usepackage[a4paper, portrait, margin=1in]{geometry}
\usepackage{centernot}

\renewcommand{\qedsymbol}{$\blacksquare$}
\renewcommand{\epsilon}{\varepsilon}

\newcommand{\R}{\mathbb{R}}
\newcommand{\Z}{\mathbb{Z}}
\newcommand{\displim}[1]{\displaystyle{\lim_{#1}\:}}
\newcommand{\zerolim}{\displim{x \to 0}}
\newcommand{\st}{\text{ s.t. }}

\newtheorem{theorem}{Theorem}

% let's begin
\begin{document}
\textbf{(Q7)}

\textit{(a)}
True.

\begin{proof}
    Formally speaking, what we are trying to prove is that:

    \begin{gather*}
        \forall \epsilon > 0,\: \exists \delta_1 > 0 \st \forall x \in \R,\\
        0 < |x - a| < \delta_1 \implies |f(x)| < \epsilon \quad (1)\\
        \text{if and only if}\\
        \forall \epsilon > 0,\: \exists \delta_2 > 0 \st \forall x \in \R,\\
        0 < |x - a| < \delta_2 \implies \left||f(x)|\right| < \epsilon \quad (2)
    \end{gather*}

    In order to prove that $(1) \iff (2)$, we have to prove that $(1) \implies (2)$
    and $(2) \implies (1)$.

    Assuming $(1)$, let $\epsilon$ be arbitrary and fix $\delta_2 = \delta_1$.
    We observe that $\left||f(x)|\right| = |f(x)|$. Thus,
    \[
        0 < |x - a| < \delta_1 \implies |f(x)| = \left||f(x)|\right|
    \]

    Which proves $(1) \implies (2)$.

    Assuming $(2)$, let $\epsilon$ be arbitrary and fix $\delta_1 = \delta_2$.
    Using the same observation,

    \[
        0 < |x - a| < \delta_2 \implies \left||f(x)|\right| = |f(x)|
    \]

    Which proves $(2) \implies (1)$.

    Since we have proven that $(1) \implies (2)$ and $(2) \implies (1)$, we can
    conclude that $(1) \iff (2)$, as required.

\end{proof}

\textit{(b)}
False.

As a counterexample, consider the function:

\[
    f(x) = \begin{cases}
        1 \text{ if $x < a$}\\
        -1 \text{ if $x > a$}
    \end{cases}
\]

$f(x)$ has no limit at $a$, while $|f(x)|$ does. In other words,

\[
    \displim{x \to a} |f(x)| = 1 \centernot\implies \displim{x \to a} f(x) = 1
\]


\end{document}