\documentclass[12pt, a4paper]{article}
\setlength{\parindent}{0pt}
\usepackage{amsmath}
\usepackage{amsthm}
\usepackage{amssymb}
\usepackage[a4paper, portrait, margin=1in]{geometry}

% i like the black square better.
\renewcommand{\qedsymbol}{$\blacksquare$}
%\renewcommand{\implies}{\Rightarrow}
\newcommand{\dispst}{\displaystyle}

\newcommand{\N}{\mathbb{N}}
\newcommand{\ddx}{\frac{d}{dx}}

\newtheorem{theorem}{Theorem}

% let's begin
\begin{document}

\textbf{(Q2)}

\textit{(a)} $(f \circ g) = (\sin x)^3$

By the Chain Rule,
\[
    \ddx (\sin x)^3 = 3(\sin x)^2 \cdot \cos x
\]

\textit{(b)} $\dispst\left(\frac{f}{g}\right) = \dispst\frac{x^3}{\sin x}$.

By the Quotient Rule,
\begin{align*}
    \ddx \left(\frac{x^3}{\sin x}\right) & = \frac{3x^2 \sin x - x^3 \cos x}{\sin^2 x}\\
    & = \frac{3x^2 \sin x}{\sin^2x} - \frac{x^3 \cos x}{\sin x}\\
    & = \frac{3x^2}{\sin x} - \left(\frac{x^3}{\sin x} \cdot \frac{\cos x}{\sin x}\right)\\
    & = 3x^2 \csc x - \left(x^3 \csc x \cdot \cot x\right)\\
    & = x^2\csc x (3 - x \cot x)
\end{align*}

\textit{(c)} $\left(2f - (h \circ g)\right) = 2x^3 - e^{\sin x}$.

By the Chain Rule,
\[
    \ddx 2x^3 - e^{\sin x} = 6x^2 - (e^{\sin x} \cos x)
\]

\textit{(d)} We observe that $(f \circ g \circ h)'(x) = f'(g(h(x))) \cdot \ddx g(h(x))$
via the Chain Rule. In turn, $\ddx g(h(x)) = g'(h(x)) \cdot h'(x)$. In all:
\[
    \ddx f(g(h(x))) = f'(g(h(x))) \cdot g'(h(x)) \cdot h'(x)
\]\

Applying this to the given functions:
\begin{align*}
    \ddx (e^{sin x})^3 & = 3(e^{sin x})^2 \cdot e^{sin x} \cdot \cos x\\
    & = 3(e^{\sin x})^3 \cdot \cos x
\end{align*}

\textit{(e)} We observe, by the Product Rule:
\begin{align*}
    (f \cdot g \cdot h)' & = f'(gh) + f(gh)'\\
    & = f'gh + f(g'h + gh')\\
    & = f'gh + fg'h + fgh'
\end{align*}

Applying this to the given functions:
\begin{align*}
    \ddx \left(x^3 \sin x e^x\right) & = (3x^2 \cdot \sin x \cdot e^x)
    + (x^3 \cdot \cos x \cdot e^x) + (x^3 \cdot \sin x \cdot e^x)\\
    & = x^2 e^x\left(3\sin x + x \cdot \cos x + x \cdot \sin x\right)\\
    & = e^x\left((3 + x)(\sin x) + x \cdot \cos x\right)
\end{align*}

\end{document}