\documentclass[12pt, a4paper]{article}
\setlength{\parindent}{0pt}
\usepackage{amsmath}
\usepackage{amsthm}
\usepackage{amssymb}
\usepackage[a4paper, portrait, margin=1in]{geometry}

% i like the black square better.
\renewcommand{\qedsymbol}{$\blacksquare$}
%\renewcommand{\implies}{\Rightarrow}
\newcommand{\dispst}{\displaystyle}

\newcommand{\R}{\mathbb{R}}
\newcommand{\ddx}{\frac{d}{dx}}

\newtheorem{theorem}{Theorem}

% let's begin
\begin{document}

\textbf{(Q4)} 

Given the curve $\sin (2x - y) + x^3y^2 + 1 = e^{y - x^2}$, we are required to find
the equation of the tangent line at $(0,0)$.

We can find the derivative by means of implicit differentiation:

\begin{gather*}
    \ddx \sin (2x - y) + x^3y^2 + 1 - e^{y - x^2}\\
    = (\cos(2x-y) \cdot 2 - y') + (3x^2y^2 + x^3(2y \cdot y')) - (e^{y-x^2} \cdot (y' - 2x))
\end{gather*}

Considering the curve at (0, 0):

\begin{gather*}
    (\cos(0) \cdot 2 - y') + (3(0)^2(0)^2 + 0^3(0 \cdot y')) - (e^{0-0^2} \cdot (y' - 0))\\
    = 2 - y' - y' = 0 \implies y' = 1
\end{gather*}

Therefore, the slope of the tangent is 1. Substituting the point (0,0) and slope into the 
form $y = mx + b$:
\begin{align*}
    0 = 1(0) + b & \implies b = 0\\
    & \implies y = x
\end{align*}

Which is the equation of the tangent line.

\end{document}