\documentclass[12pt, a4paper]{article}
\setlength{\parindent}{0pt}
\usepackage{amsmath}
\usepackage{amsthm}
\usepackage{amssymb}
\usepackage[a4paper, portrait, margin=1in]{geometry}

% i like the black square better.
\renewcommand{\qedsymbol}{$\blacksquare$}
\newcommand{\dispst}{\displaystyle}

\newcommand{\ddx}{\frac{d}{dx}}

\begin{document}

\textbf{(Q6)}

\begin{proof}
    We aim to prove the implication:
    \[
        f(-x) = f(x) \implies f'(-x) = -f'(x)
    \]

    Assuming that $f$ is even (i.e. $f(x) = f(-x)$), it then follows:
    \begin{align*}
        \ddx f(x) = \ddx f(-x) & \implies f'(x) = -1 \cdot f'(-x) \text{ (by Chain Rule)}\\
        & \implies f'(x) = -f'(-x)\\
        & \implies -f'(x) = f'(-x)
    \end{align*}

    By the given definition of a odd function, we have proven that if $f$ is even,
    then $f'$ is odd, as required.
\end{proof}
\end{document}