\documentclass[12pt, a4paper]{article}
\setlength{\parindent}{0pt}
\usepackage{amsmath}
\usepackage{amsthm}
\usepackage{amssymb}
\usepackage[a4paper, portrait, margin=1in]{geometry}

% i like the black square better.
\renewcommand{\qedsymbol}{$\blacksquare$}
%\renewcommand{\implies}{\Rightarrow}

\newcommand{\N}{\mathbb{N}}
\newcommand{\Q}{\mathbb{Q}}

\newcommand{\ddx}{\frac{d}{dx}}
\newcommand{\st}{\; \colon \;}
\newcommand{\sse}{\subseteq}
\newcommand{\lsum}[2]{L_{#1}(#2)}
\newcommand{\usum}[2]{U_{#1}(#2)}

\newtheorem{theorem}{Theorem}

% let's begin
\begin{document}

\textbf{(Q7)}

\begin{theorem}
    For any bounded function $f, g$ and partition $P$ of $[a, b]$, we have
    \[\usum{P}{f + g} \geq \usum{P}{f} + \usum{P}{g}\]
\end{theorem}

\begin{proof}
    For convenience, let $I = [a, b]$ and $\Delta_a = b - a$. We observe that
    \begin{gather*}
        \sup\{(f + g)(I)\} \geq \sup\{f(I)\} + \sup\{g(I)\}\\
        \Downarrow\\
        \sup\{(f + g)(I)\}\Delta_a \geq \sup\{f(I)\}\Delta_a + \sup\{g(I)\}\Delta_a \quad (1)
    \end{gather*}

    Therefore, for any partition $P = \{x_0, x_1, \ldots x_n\}$ of $[a, b]$:
    \begin{gather*}
        \usum{P}{f} = \sum_{i = 1}^{n} \sup f([x_{i - 1}, x_i]) \cdot (x_i - x_{i - 1})\\
        \usum{P}{g} = \sum_{i = 1}^{n} \sup g([x_{i - 1}, x_i]) \cdot (x_i - x_{i - 1})\\
        \usum{P}{f + g} = \sum_{i = 1}^{n} \sup (f + g)([x_{i - 1}, x_i]) \cdot (x_i - x_{i - 1})
    \end{gather*}

    Since (1) holds for every term in the summation, we can conclude that:
    \[
        \usum{P}{f + g} \geq \usum{P}{f} + \usum{P}{g}
    \]
\end{proof}

\end{document}