\documentclass[12pt, a4paper]{article}
\setlength{\parindent}{0pt}
\usepackage[a4paper, portrait, margin=1in]{geometry}
\usepackage{graphicx}

\graphicspath{.}

\usepackage{preamble}

\begin{document}
\textbf{Q1}

\textit{(a)}

We first manipulate the rational into something easier to work with:
\begin{align*}
    \frac{x^2}{x^2 + 9} & = \frac{A}{x^2 + 9} + \frac{x^2 + 9}{x^2 + 9}\\
    & = \frac{-9}{x^2 + 9}
\end{align*}
Using substitution, let $u = \frac{x}{3}, du = \frac{1}{3}dx$. Then
\begin{align*}
    -3 \int \frac{1}{\frac{x^2}{9} + 1} \cdot \frac{1}{3} dx
    & = -3 \int \frac{1}{u^2 + 1} du\\
    & = -3 \arctan(u) \\ & = -3 \arctan(\frac{x}{3}) + c
\end{align*}

\textit{(b)}

We manipulate the rational into something easier to work with:

\begin{align*}
    \frac{x^2}{x^2+2x+2} & = \frac{A}{x^2 + 2x + 2} + 1\\
    & = \frac{-2x - 2}{x^2 + 2x + 2} + 1
\end{align*}

Then 
\begin{align*}
    \int \frac{x^2}{x^2 + 2x + 2}dx
    & = \int \left(\frac{-2x - 2}{x^2 + 2xc + 2} + 1\right)dx\\
    & = -\int \left((2x + 2)\cdot\frac{1}{x^2 + 2xc + 2} + 1\right)dx
\end{align*}
Using the substitution $u = x^2 + 2x +2, du = (2x + 2) dx$, then
\begin{align*}
    - \int \frac{1}{u} du + \int 1 dx & = \ln |u| + x\\
    & = -\ln |x^2 + 2x + 2| + x + c
\end{align*}
\end{document}